example/FailOnReentrance.thy
@@ -124,11 +124,13 @@ where
      venv_storage_at_call ve 0 = 0 \<Longrightarrow>
      fail_on_reentrance_invariant st"
      
-value "program_of_lst fail_on_reentrance_program"
+value "program_content (program_of_lst fail_on_reentrance_program program_content_of_lst) 8"
 
 declare one_round.simps [simp]
 declare world_turn.simps [simp]
 declare contract_turn.simps [simp]
+
+declare to_bl_def [simp]
 
 lemma invariant_kept:
 "no_assertion_failure fail_on_reentrance_invariant"
