lem/Lem.thy
@@ -1,0 +1,110 @@
+(*** This file is part of Lem.  eth-isabelle project just uses it.  See lem-license. ***)
+
+(*========================================================================*)
+(*                        Lem                                             *)
+(*                                                                        *)
+(*          Dominic Mulligan, University of Cambridge                     *)
+(*          Francesco Zappa Nardelli, INRIA Paris-Rocquencourt            *)
+(*          Gabriel Kerneis, University of Cambridge                      *)
+(*          Kathy Gray, University of Cambridge                           *)
+(*          Peter Boehm, University of Cambridge (while working on Lem)   *)
+(*          Peter Sewell, University of Cambridge                         *)
+(*          Scott Owens, University of Kent                               *)
+(*          Thomas Tuerk, University of Cambridge                         *)
+(*                                                                        *)
+(*  The Lem sources are copyright 2010-2013                               *)
+(*  by the UK authors above and Institut National de Recherche en         *)
+(*  Informatique et en Automatique (INRIA).                               *)
+(*                                                                        *)
+(*  All files except ocaml-lib/pmap.{ml,mli} and ocaml-libpset.{ml,mli}   *)
+(*  are distributed under the license below.  The former are distributed  *)
+(*  under the LGPLv2, as in the LICENSE file.                             *)
+(*                                                                        *)
+(*                                                                        *)
+(*  Redistribution and use in source and binary forms, with or without    *)
+(*  modification, are permitted provided that the following conditions    *)
+(*  are met:                                                              *)
+(*  1. Redistributions of source code must retain the above copyright     *)
+(*  notice, this list of conditions and the following disclaimer.         *)
+(*  2. Redistributions in binary form must reproduce the above copyright  *)
+(*  notice, this list of conditions and the following disclaimer in the   *)
+(*  documentation and/or other materials provided with the distribution.  *)
+(*  3. The names of the authors may not be used to endorse or promote     *)
+(*  products derived from this software without specific prior written    *)
+(*  permission.                                                           *)
+(*                                                                        *)
+(*  THIS SOFTWARE IS PROVIDED BY THE AUTHORS ``AS IS'' AND ANY EXPRESS    *)
+(*  OR IMPLIED WARRANTIES, INCLUDING, BUT NOT LIMITED TO, THE IMPLIED     *)
+(*  WARRANTIES OF MERCHANTABILITY AND FITNESS FOR A PARTICULAR PURPOSE    *)
+(*  ARE DISCLAIMED. IN NO EVENT SHALL THE AUTHORS BE LIABLE FOR ANY       *)
+(*  DIRECT, INDIRECT, INCIDENTAL, SPECIAL, EXEMPLARY, OR CONSEQUENTIAL    *)
+(*  DAMAGES (INCLUDING, BUT NOT LIMITED TO, PROCUREMENT OF SUBSTITUTE     *)
+(*  GOODS OR SERVICES; LOSS OF USE, DATA, OR PROFITS; OR BUSINESS         *)
+(*  INTERRUPTION) HOWEVER CAUSED AND ON ANY THEORY OF LIABILITY, WHETHER  *)
+(*  IN CONTRACT, STRICT LIABILITY, OR TORT (INCLUDING NEGLIGENCE OR       *)
+(*  OTHERWISE) ARISING IN ANY WAY OUT OF THE USE OF THIS SOFTWARE, EVEN   *)
+(*  IF ADVISED OF THE POSSIBILITY OF SUCH DAMAGE.                         *)
+(*========================================================================*)
+
+header{* Mappings of Syntax needed by Lem *}
+
+theory "Lem" 
+
+imports 
+ 	 Main
+         LemExtraDefs
+         "~~/src/HOL/Map"
+         "~~/src/HOL/Library/Code_Target_Numeral"
+
+begin 
+
+type_synonym numeral = nat
+
+subsection{* Finite Maps *}
+
+abbreviation (input) "map_find k m \<equiv> the (m k)"
+abbreviation (input) "map_update k v m \<equiv> m (k \<mapsto> v)"
+abbreviation (input) "map_remove k m \<equiv> m |` (- {k})"
+abbreviation (input) "map_any P m \<equiv> \<exists> (k, v) \<in> map_to_set m. P k v"
+abbreviation (input) "map_all P m \<equiv> \<forall> (k, v) \<in> map_to_set m. P k v"
+
+subsection{* Lists *}
+
+abbreviation (input) "list_mem e l \<equiv> (e \<in> set l)"
+abbreviation (input) "list_forall P l \<equiv> (\<forall>e\<in>set l. P e)"
+abbreviation (input) "list_exists P l \<equiv> (\<exists>e\<in>set l. P e)"
+abbreviation (input) "list_unzip l \<equiv> (map fst l, map snd l)"
+
+subsection{* Sets *}
+
+abbreviation (input) "set_filter P (s::'a set) \<equiv> {x \<in> s. P x}"
+abbreviation (input) "set_bigunion S \<equiv> \<Union> S"
+abbreviation (input) "set_biginter S \<equiv> \<Inter> S"
+
+subsection{* Natural numbers *}
+
+subsection{* Integers *}
+
+
+subsection {* Dummy *}
+
+definition bitwise_xor :: "nat \<Rightarrow> nat \<Rightarrow> nat" where
+  "bitwise_xor x y = undefined"
+
+definition num_asr :: "nat \<Rightarrow> nat \<Rightarrow> nat" where
+  "num_asr n m = undefined"
+
+definition num_lsl :: "nat \<Rightarrow> nat \<Rightarrow> nat" where
+  "num_lsl n m = undefined"
+
+definition bitwise_or :: "nat \<Rightarrow> nat \<Rightarrow> nat" where
+  "bitwise_or n m = undefined"
+
+definition bitwise_not :: "nat \<Rightarrow> nat" where
+  "bitwise_not n = undefined"
+
+definition bitwise_and :: "nat \<Rightarrow> nat \<Rightarrow> nat" where
+  "bitwise_and n m = undefined"
+
+
+end
