README.md
@@ -18,7 +18,7 @@ When you see `\<Rightarrow>` in the source, try using the [Isabelle2016](https:/
 ## Makefile goals
 
 * `make deed` produces a verified PDF document for the Deed contract
-* `make lem-check` compiles the Lem sources into Isabelle/HOL
+* `make lem-thy` compiles the Lem sources into Isabelle/HOL
 * `make all-isabelle` checks all Isabelle/HOL sources (but not the ones compiled from Lem)
 * `make` does everything above
 
